examples/iterators/DupElementsMap.dfy
@@ -4,6 +4,7 @@ include "../../src/linear/layer2/ArrayList.dfy"
 include "Dup_Utils.dfy"
 include "../../src/Iterators_Utils.dfy"
 
+//Con BuildMap hace falta {:timeLimitMultiplier 10}
 
 method DupElements<A>(l: LinkedList<A>) returns (ghost mit:map<int,int>)
   modifies l, l.Repr()
@@ -20,18 +21,18 @@ method DupElements<A>(l: LinkedList<A>) returns (ghost mit:map<int,int>)
   ensures l.Iterators() >= old(l.Iterators())
   ensures forall it | it in old(l.Iterators()) && old(it.Valid()) && old(it.Index()) in mit::
      it.Valid() && it.Parent()==old(it.Parent()) && mit[old(it.Index())]==it.Index()
-  ensures mit== dupMap(old(l.Model()),|old(l.Model())|)
-  //ensures mit == buildMap((set it |it in old(l.Iterators()) && old(it.Valid())::old(it.Index())),fdup(|old(l.Model())|))
+  ensures mit== DupMapI(old(l.Model()),|old(l.Model())|)
+  //ensures mit == BuildMap((set it |it in old(l.Iterators()) && old(it.Valid())::old(it.Index())),DupF(|old(l.Model())|))
   ensures forall it | it in old(l.Iterators()) && old(it.Valid()):: old(it.Index()) in mit //domain
-  ensures forall i | i in mit :: mit[i]==dup(i,|old(l.Model())|)//range
+  ensures forall i | i in mit :: mit[i]==DupI(i,|old(l.Model())|)//range
 {
 
     //ghost var validSet:=(set it |it in old(l.Iterators()) && old(it.Valid())::old(it.Index()));
-    //mit:=buildMap(validSet,identity);
-     mit:= dupMap(old(l.Model()),0);
+    //mit:=BuildMap(validSet,Identity);
+    mit:= DupMapI(old(l.Model()),0);
 
-  var it := l.Begin();
-  var b := it.HasNext();  
+  var it := l.First();
+  var b := it.HasPeek();  
    
   ghost var i := 0;
   
@@ -43,25 +44,26 @@ method DupElements<A>(l: LinkedList<A>) returns (ghost mit:map<int,int>)
     invariant l.Valid()
     invariant 2*i <= |l.Model()|
     invariant i <= old(|l.Model()|)
-    invariant l.Model()[..2*i] == old(DupRev(l.Model()[..i]))
+    invariant l.Model()[..2*i] == DupRev(old(l.Model()[..i]))
     invariant l.Model()[2*i..] == old(l.Model()[i..])
     invariant it.Parent() == l
     invariant it.Valid()
     invariant {it} !! {l}
     invariant it.Index() == 2*i
     invariant it in l.Iterators()
-    invariant b == it.HasNext?()
+    invariant b == it.HasPeek?()
 
     invariant l.Iterators() >= old(l.Iterators())
     invariant forall iter | iter in old(l.Iterators()) && old(iter.Valid()) && old(iter.Index()) in mit::
        iter.Valid() && iter.Parent()==old(iter.Parent()) && mit[old(iter.Index())]==iter.Index()
-    //invariant  mit == buildMap((set it |it in old(l.Iterators()) && old(it.Valid())::old(it.Index())),fdupInvariant(i))
-    invariant mit== dupMap(old(l.Model()),i)
+    //invariant it !in old(l.Iterators())
+    //invariant  mit == BuildMap((set it |it in old(l.Iterators()) && old(it.Valid())::old(it.Index())),DupInvariantF(i))
+    invariant mit== DupMapI(old(l.Model()),i)
   {
 
     assert i < old(|l.Model()|);
     ghost var omodel := l.Model();
-    assert omodel[..2*i] == old(DupRev(l.Model()[..i]));
+    assert omodel[..2*i] == DupRev(old(l.Model()[..i]));
     assert omodel[2*i]==old(l.Model()[i]);
 
     var x := it.Peek();
@@ -85,28 +87,23 @@ method DupElements<A>(l: LinkedList<A>) returns (ghost mit:map<int,int>)
      }
      assert model == DupRev(old(l.Model()[..i+1])) + omodel[2*i+1..];
 
-    var _ := it.Next();
-    b := it.HasNext();
+    it.Next();
+    b := it.HasPeek();
     i := i + 1;
     
-     // mit:=buildMap(validSet,fdupInvariant(i));
-     mit:=dupMap(old(l.Model()),i);
-    }
+    //mit:=BuildMap(validSet,DupInvariantF(i));
+    mit:=DupMapI(old(l.Model()),i);
+  }
  
- //mit:=buildMap(validSet,fdup(|old(l.Model())|));
+ //mit:=BuildMap(validSet,DupF(|old(l.Model())|));
   
   assert i==|old(l.Model())|;
   DupDupRev(old(l.Model()[..i]));
   assert old(l.Model()[..i]) == old(l.Model());
   //assert l.Model() == old(Dup(l.Model()));
-  setDup(old(l.Model())); // 0->0,1 1-> 2,3 ...
+  SetDup(old(l.Model())); // 0->0,1 1-> 2,3 ...
 
 }
-
-
-
-
-
 
 
 method DupElementsAL(l: ArrayList<int>) returns (ghost mit:map<int,int>)
@@ -124,17 +121,17 @@ method DupElementsAL(l: ArrayList<int>) returns (ghost mit:map<int,int>)
   ensures l.Iterators() >= old(l.Iterators())
   ensures forall it | it in old(l.Iterators()) && old(it.Valid()) && old(it.Index()) in mit::
       it.Valid() && it.Parent()==old(it.Parent()) && mit[old(it.Index())]==it.Index()
-  ensures mit == buildMap((set it |it in old(l.Iterators()) && old(it.Valid())::old(it.Index())),identity)
+  ensures mit == BuildMap((set it |it in old(l.Iterators()) && old(it.Valid())::old(it.Index())),Identity)
   ensures forall it | it in old(l.Iterators()) && old(it.Valid()):: old(it.Index()) in mit //domain
-  ensures forall i | i in mit :: mit[i]==identity(i)//range
+  ensures forall i | i in mit :: mit[i]==Identity(i)//range
 {
      
     ghost var validSet:=(set it |it in old(l.Iterators()) && old(it.Valid())::old(it.Index()));
-    mit:=buildMap(validSet,identity);
+    mit:=BuildMap(validSet,Identity);
 
 
-  var it := l.Begin();
-  var b := it.HasNext();
+  var it := l.First();
+  var b := it.HasPeek();
 
   ghost var i := 0;
   
@@ -153,7 +150,7 @@ method DupElementsAL(l: ArrayList<int>) returns (ghost mit:map<int,int>)
     invariant {it} !! {l}
     invariant it.Index() == 2*i
     invariant it in l.Iterators()
-    invariant b == it.HasNext?()
+    invariant b == it.HasPeek?()
 
     invariant l.Iterators() >= old(l.Iterators())
     invariant it !in old(l.Iterators())
@@ -187,9 +184,9 @@ method DupElementsAL(l: ArrayList<int>) returns (ghost mit:map<int,int>)
     assert model == DupRev(old(l.Model()[..i+1])) + omodel[2*i+1..];
 
 
-    var _ := it.Next();
-    var _ := it.Next(); //In ArrayList index mid remains, so we jump over two elements to reach the following one
-    b := it.HasNext();
+    it.Next();
+    it.Next(); //In ArrayList index mid remains, so we jump over two elements to reach the following one
+    b := it.HasPeek();
     i := i + 1;
 
 
@@ -200,11 +197,11 @@ method DupElementsAL(l: ArrayList<int>) returns (ghost mit:map<int,int>)
   assert old(l.Model()[..i]) == old(l.Model());
 
   //assert l.Model() == old(Dup(l.Model()));
-  setDup(old(l.Model())); // 0->0,1 1-> 2,3 ...
+  SetDup(old(l.Model())); // 0->0,1 1-> 2,3 ...
 
 }
 
-method dupDup<A>(l:LinkedList<A>)returns (ghost mit:map<int,int>)
+method DupDup<A>(l:LinkedList<A>)returns (ghost mit:map<int,int>)
 modifies l, l.Repr()
   requires l.Valid()
   requires forall x | x in l.Repr() :: allocated(x)
@@ -235,8 +232,8 @@ modifies l, l.Repr()
 
   ensures l.Iterators() >= old(l.Iterators())
 {
-  var it := l.Begin();
-  var b := it.HasNext();
+  var it := l.First();
+  var b := it.HasPeek();
 
   ghost var i := 0;
   
@@ -255,7 +252,7 @@ modifies l, l.Repr()
     invariant {it} !! {l}
     invariant it.Index() == 2*i
     invariant it in l.Iterators()
-    invariant b == it.HasNext?()
+    invariant b == it.HasPeek?()
 
     invariant l.Iterators() >= old(l.Iterators())
     invariant it !in old(l.Iterators())
@@ -287,9 +284,9 @@ modifies l, l.Repr()
     assert model == DupRev(old(l.Model()[..i+1])) + omodel[2*i+1..];
 
 
-    var _ := it.Next();
-    var _ := it.Next(); 
-    b := it.HasNext();
+    it.Next();
+    it.Next(); 
+    b := it.HasPeek();
     i := i + 1;
 
 
@@ -300,6 +297,6 @@ modifies l, l.Repr()
   assert old(l.Model()[..i]) == old(l.Model());
 
   //assert l.Model() == old(Dup(l.Model()));
-  setDup(old(l.Model())); // 0->0,1 1-> 2,3 ...
+  SetDup(old(l.Model())); // 0->0,1 1-> 2,3 ...
 
 }
