examples/iterators/FillArrayMap.dfy
@@ -21,13 +21,13 @@ method FillArrayLL<A>(l: LinkedList<A>, v: array<A>) returns (ghost mit:map<int,
   ensures l.Iterators() >= old(l.Iterators())
   ensures forall it | it in old(l.Iterators()) && old(it.Valid()) && old(it.Index()) in mit::
      it.Valid() && it.Parent()==old(it.Parent()) && mit[old(it.Index())]==it.Index()
-  ensures mit==identityMap((set it |it in old(l.Iterators()) && old(it.Valid())::old(it.Index())))
+  ensures mit==IdentityMap((set it |it in old(l.Iterators()) && old(it.Valid())::old(it.Index())))
   //ensures mit==buildMap((set it |it in old(l.Iterators()) && old(it.Valid())::old(it.Index())),identity)
   ensures forall it | it in old(l.Iterators()) && old(it.Valid()):: old(it.Index()) in mit //domain
-  ensures forall i | i in mit :: mit[i]==identity(i) //range
+  ensures forall i | i in mit :: mit[i]==Identity(i) //range
 {
   var validSet := set it |it in old(l.Iterators()) && old(it.Valid())::old(it.Index());
-  mit := identityMap(validSet);
+  mit := IdentityMap(validSet);
 
   var it := l.First();
   var b := it.HasPeek();
@@ -78,13 +78,13 @@ method FillArrayAL<A>(l: ArrayList<A>, v: array<A>)returns (ghost mit:map<int,in
   ensures l.Iterators() >= old(l.Iterators())
   ensures forall it | it in old(l.Iterators()) && old(it.Valid()) && old(it.Index()) in mit::
      it.Valid() && it.Parent()==old(it.Parent()) && mit[old(it.Index())]==it.Index()
-  ensures mit==identityMap((set it |it in old(l.Iterators()) && old(it.Valid())::old(it.Index())))
+  ensures mit==IdentityMap((set it |it in old(l.Iterators()) && old(it.Valid())::old(it.Index())))
   //ensures mit==buildMap((set it |it in old(l.Iterators()) && old(it.Valid())::old(it.Index())),identity)
   ensures forall it | it in old(l.Iterators()) && old(it.Valid()):: old(it.Index()) in mit //domain
-  ensures forall i | i in mit :: mit[i]==identity(i) //range
+  ensures forall i | i in mit :: mit[i]==Identity(i) //range
 {
   var validSet:=set it |it in old(l.Iterators()) && old(it.Valid())::old(it.Index());
-  mit:=identityMap(validSet);
+  mit:=IdentityMap(validSet);
 
   var it := l.First();
   var b := it.HasPeek();
